trace_index → ordinal

dimsum/iris/mono_ord.v
@@ -1,12 +1,12 @@
 From iris.algebra Require Export cmra local_updates proofmode_classes auth.
 From iris.algebra Require Import updates.
 From iris.prelude Require Import options.
-From dimsum.core Require Export trace_index.
+From dimsum.core Require Export ordinal.
 
 (** This file is based min_nat in iris/algebra/numbers.v and mono_nat in iris/algebra/lib/mono_nat.v . *)
 
 (** ** Ordinals with [min] as the operation. *)
-Record min_ord := MinOrd { min_ord_car : trace_index }.
+Record min_ord := MinOrd { min_ord_car : ordinal }.
 Add Printing Constructor min_ord.
 
 Global Instance min_ord_equiv : Equiv min_ord := λ x y, min_ord_car x ≡ min_ord_car y.
@@ -18,26 +18,26 @@ Proof. move => ???. done. Qed.
 Canonical Structure min_ordO := discreteO min_ord.
 
 Section min_ord.
-  Local Instance min_ord_unit_instance : Unit min_ord := MinOrd (tiChoice Empty_set (λ x, match x with end)) .
+  Local Instance min_ord_unit_instance : Unit min_ord := MinOrd (oChoice Empty_set (λ x, match x with end)) .
   Local Instance min_ord_valid_instance : Valid min_ord := λ x, True.
   Local Instance min_ord_validN_instance : ValidN min_ord := λ n x, True.
   Local Instance min_ord_pcore_instance : PCore min_ord := Some.
-  Local Instance min_ord_op_instance : Op min_ord := λ n m, MinOrd (ti_min (min_ord_car n) (min_ord_car m)).
-  Definition min_ord_op_min x y : MinOrd x ⋅ MinOrd y = MinOrd (ti_min x y) := eq_refl.
+  Local Instance min_ord_op_instance : Op min_ord := λ n m, MinOrd (o_min (min_ord_car n) (min_ord_car m)).
+  Definition min_ord_op_min x y : MinOrd x ⋅ MinOrd y = MinOrd (o_min x y) := eq_refl.
 
   Lemma min_ord_included (x y : min_ord) : x ≼ y ↔ min_ord_car y ⊆ min_ord_car x.
   Proof.
     split.
-    - intros [z [-> ?]]. simpl. apply ti_min_le_l.
-    - exists y. rewrite /op /min_ord_op_instance. symmetry. by apply ti_min_r.
+    - intros [z [-> ?]]. simpl. apply o_min_le_l.
+    - exists y. rewrite /op /min_ord_op_instance. symmetry. by apply o_min_r.
   Qed.
   Lemma min_ord_ra_mixin : RAMixin min_ord.
   Proof.
     apply ra_total_mixin; apply _ || eauto.
     - intros [x] [?] [?] Heq. rewrite !min_ord_op_min. rewrite /equiv/min_ord_equiv/= in Heq. by rewrite Heq.
-    - intros [x] [y] [z]. repeat rewrite min_ord_op_min. by apply ti_min_assoc.
-    - intros [x] [y]. rewrite !min_ord_op_min. apply ti_min_comm.
-    - intros [x]. rewrite min_ord_op_min. apply ti_min_id.
+    - intros [x] [y] [z]. repeat rewrite min_ord_op_min. by apply o_min_assoc.
+    - intros [x] [y]. rewrite !min_ord_op_min. apply o_min_comm.
+    - intros [x]. rewrite min_ord_op_min. apply o_min_id.
   Qed.
   Canonical Structure min_ordR : cmra := discreteR min_ord min_ord_ra_mixin.
 
@@ -58,21 +58,21 @@ Section min_ord.
     rewrite 2!min_ord_op_min. intros [Heq1 Heq2]; simpl in *.
     split; first done. rewrite ->Heq1 in Hle.
     split => /=.
-    - apply ti_min_l_2. rewrite Hle. apply ti_min_le_r.
-    - apply ti_min_le_l.
+    - apply o_min_l_2. rewrite Hle. apply o_min_le_r.
+    - apply o_min_le_l.
   Qed.
 
-  Global Instance : LeftAbsorb (≡) (MinOrd tiO) (⋅).
-  Proof. move => [x]. rewrite min_ord_op_min. apply ti_min_l. constructor. Qed.
+  Global Instance : LeftAbsorb (≡) (MinOrd oO) (⋅).
+  Proof. move => [x]. rewrite min_ord_op_min. apply o_min_l. constructor. Qed.
 
-  Global Instance : RightAbsorb (≡) (MinOrd tiO) (⋅).
-  Proof. move => [x]. rewrite min_ord_op_min. apply ti_min_r. constructor. Qed.
+  Global Instance : RightAbsorb (≡) (MinOrd oO) (⋅).
+  Proof. move => [x]. rewrite min_ord_op_min. apply o_min_r. constructor. Qed.
 
   Global Instance : IdemP (≡@{min_ord}) (⋅).
-  Proof. intros [x]. rewrite min_ord_op_min. apply ti_min_id. Qed.
+  Proof. intros [x]. rewrite min_ord_op_min. apply o_min_id. Qed.
 
   Global Instance min_ord_is_op x y :
-    IsOp (MinOrd (ti_min x y)) (MinOrd x) (MinOrd y).
+    IsOp (MinOrd (o_min x y)) (MinOrd x) (MinOrd y).
   Proof. done. Qed.
 End min_ord.
 
@@ -87,12 +87,12 @@ Definition mono_ordUR := authUR (optionUR min_ordR).
 fragment at the same value so that lemma [mono_ord_included], which states that
 [mono_ord_ub n ≼ mono_ord_auth q n], does not require a frame-preserving
 update. *)
-Definition mono_ord_auth (q : Qp) (n : trace_index) : mono_ord :=
+Definition mono_ord_auth (q : Qp) (n : ordinal) : mono_ord :=
   ●{#q} Some (MinOrd n) ⋅ ◯ Some (MinOrd n).
-Definition mono_ord_ub (n : trace_index) : mono_ord := ◯ Some (MinOrd n).
+Definition mono_ord_ub (n : ordinal) : mono_ord := ◯ Some (MinOrd n).
 
 Section mono_ord.
-  Implicit Types (n : trace_index).
+  Implicit Types (n : ordinal).
 
   Global Instance mono_ord_ub_core_id n : CoreId (mono_ord_ub n).
   Proof. apply _. Qed.
@@ -106,7 +106,7 @@ Section mono_ord.
   Qed.
 
   Lemma mono_ord_ub_op n1 n2 :
-    mono_ord_ub n1 ⋅ mono_ord_ub n2 = mono_ord_ub (ti_min n1 n2).
+    mono_ord_ub n1 ⋅ mono_ord_ub n2 = mono_ord_ub (o_min n1 n2).
   Proof. rewrite -auth_frag_op -Some_op min_ord_op_min //. Qed.
 
   Lemma mono_ord_auth_ub_op q n :
@@ -114,7 +114,7 @@ Section mono_ord.
   Proof.
     rewrite /mono_ord_auth /mono_ord_ub.
     rewrite -!assoc -auth_frag_op -Some_op min_ord_op_min.
-    do 3 f_equiv. symmetry. apply ti_min_id.
+    do 3 f_equiv. symmetry. apply o_min_id.
   Qed.
 
   (** rephrasing of [mono_ord_ub_op] useful for weakening a fragment to a
@@ -122,7 +122,7 @@ Section mono_ord.
   Lemma mono_ord_ub_op_le_l n n' :
     n ⊆ n' →
     mono_ord_ub n ≡ mono_ord_ub n' ⋅ mono_ord_ub n.
-  Proof. intros. rewrite mono_ord_ub_op /mono_ord_ub. do 2 f_equiv. symmetry. by apply ti_min_r. Qed.
+  Proof. intros. rewrite mono_ord_ub_op /mono_ord_ub. do 2 f_equiv. symmetry. by apply o_min_r. Qed.
 
   Lemma mono_ord_auth_frac_valid q n : ✓ mono_ord_auth q n ↔ (q ≤ 1)%Qp.
   Proof.
@@ -150,8 +150,8 @@ Section mono_ord.
     rewrite /mono_ord_auth /mono_ord_ub -assoc -auth_frag_op -Some_op.
     rewrite auth_both_dfrac_valid_discrete Some_included_total min_ord_included /=.
     split.
-    - move => [?[??]]. split; [done|]. etrans; [done|]. apply ti_min_le_r.
-    - move => [??]. split; [done|]. split; [|done]. by apply ti_min_l_2.
+    - move => [?[??]]. split; [done|]. etrans; [done|]. apply o_min_le_r.
+    - move => [??]. split; [done|]. split; [|done]. by apply o_min_l_2.
   Qed.
   Lemma mono_ord_both_valid n m :
     ✓ (mono_ord_auth 1 n ⋅ mono_ord_ub m) ↔ n ⊆ m.
