build.sh
@@ -1,4 +1,4 @@
 #!/bin/bash
 
 make -j8
-# sed -i "s/\bVisNoAll\b/VisNoAng/g" README.md dimsum/*.v dimsum_examples/*.v dimsum_examples/compiler/*.v
+# sed -i "s/\bti_not_le/o_not_le/g" README.md dimsum/*.v dimsum/iris/*.v dimsum_examples/*.v dimsum_examples/compiler/*.v
